src/Repr/SystemFOp/Kind.v
@@ -1,0 +1,8 @@
+Require Import List.
+Require Import Repr.Lists.
+
+Inductive kind : Type :=
+  | KStar : kind .
+
+Definition kenv := list kind.
+Hint Unfold kenv.
