src/Repr/SystemFOp/Syntax.v
@@ -1,0 +1,527 @@
+Require Import List.
+
+Require Import Repr.Lists.
+
+Require Import Repr.Tactics.All.
+Require Import Repr.Tactics.Rewrite.
+Require Import Repr.Tactics.Burn.
+Require Import Repr.Tactics.Norm.
+Require Import Repr.Tactics.LibTactics.
+
+Require Import Coq.Arith.Peano_dec.
+Require Import Coq.Arith.Compare_dec.
+Require Import Coq.Arith.Lt.
+
+Definition var := nat.
+Definition env := list typ.
+
+Inductive term : Set :=
+  | NConst : nat -> term
+  | Add : term -> term -> term
+
+  (* The pure lambda calculus *)                      
+  | Var : var -> term
+  | Abs : typ -> term -> term 
+  | App : term -> term -> term 
+
+  (* System F Extn *)
+  | TyAbs : term -> term
+  | TyApp : term -> typ -> term .
+                            
+Hint Constructors term.
+
+Example id_tm := (TyAbs (Abs (TVar 0) (Var 0))).
+
+Fixpoint tm_lift (dp:nat)(t:term) : term :=
+  match t with
+    | NConst n =>
+       NConst n
+    | Add t1 t2 =>
+       Add (tm_lift dp t1) (tm_lift dp t2)
+    | Var x =>
+       if (le_gt_dec dp x) then Var (S x) else Var x
+    | Abs ty t =>
+       Abs ty (tm_lift (S dp) t)
+    | App t1 t2 =>
+       App (tm_lift dp t1) (tm_lift dp t2) 
+    | TyAbs t =>
+       TyAbs (tm_lift dp t)
+    | TyApp t ty =>
+       TyApp (tm_lift dp t) ty
+   end.
+
+Fixpoint tm_substitute (x:var)(s t:term) : term :=
+  match t with
+    | NConst n => 
+       NConst n
+    | Add t1 t2 => 
+       Add (tm_substitute x s t1) (tm_substitute x s t2)
+    | Var y => 
+       match nat_compare y x with
+         | Eq => s
+         | Gt => Var (y-1)
+         | Lt => Var y
+       end
+    | Abs ty t' =>
+       Abs ty (tm_substitute (S x) (tm_lift 0 s) t')
+    | App t1 t2 =>
+       App (tm_substitute x s t1) (tm_substitute x s t2)
+    | TyAbs t' =>
+       TyAbs (tm_substitute x s t')
+    | TyApp t' ty =>
+       TyApp (tm_substitute x s t') ty
+  end.
+
+
+Fixpoint ty_tm_lift (dp:nat)(t:term) : term :=
+  match t with
+    | NConst n =>
+       NConst n
+    | Add t1 t2 =>
+       Add (ty_tm_lift dp t1) (ty_tm_lift dp t2)
+    | Var x =>
+       Var x
+    | Abs ty t =>
+       Abs (ty_lift dp ty) ((ty_tm_lift dp) t)
+    | App t1 t2 =>
+       App (ty_tm_lift dp t1) (ty_tm_lift dp t2) 
+    | TyAbs t =>
+       TyAbs (ty_tm_lift (S dp) t)
+    | TyApp t ty =>
+       TyApp (ty_tm_lift dp t) (ty_lift dp ty)
+   end.
+
+Fixpoint ty_tm_substitute (X:tvar)(S:typ)(t:term) : term :=
+  match t with
+    | NConst n => 
+       NConst n
+    | Add t1 t2 => 
+       Add (ty_tm_substitute X S t1) (ty_tm_substitute X S t2)
+    | Var y => 
+       Var y
+    | Abs ty t' =>
+       Abs (ty_substitute X S ty) (ty_tm_substitute X S t')
+    | App t1 t2 =>
+       App (ty_tm_substitute X S t1) (ty_tm_substitute X S t2)
+    | TyAbs t' =>
+       TyAbs (ty_tm_substitute X S t')
+    | TyApp t' ty =>
+       TyApp (ty_tm_substitute X S t') (ty_substitute X S ty)
+  end.
+
+Fixpoint env_substitute (X:tvar)(U:typ)(G:env) : env :=
+  match G with
+    | nil           => nil
+    | (tag,T) :: G' => (tag, (ty_substitute X U T)) :: env_substitute X U G'
+  end.
+
+Fixpoint env_lift (dp:nat)(G:env) : env :=
+  match G with
+    | nil     => nil
+    | (tag,T) :: G' => (tag, ty_lift dp T) :: env_lift dp G'
+  end.
+
+Notation "'[' x '~>' s ']' t" := (tm_substitute x s t) (at level 30).
+Notation "'[' X '~~>' S ']' t" := (ty_tm_substitute X S t) (at level 30).
+Notation "'[' X '^>' S ']' T" := (ty_substitute X S T) (at level 30).
+Notation "'[' X '^^>' S ']' G" := (env_substitute X S G) (at level 30).
+
+Inductive weak_normal : term -> Prop :=
+  | WN_NConst : 
+      forall n, weak_normal (NConst n)
+  | WN_Var :
+      forall x, weak_normal (Var x)
+  | WN_Abs :
+      forall t ty, weak_normal (Abs ty t) 
+  | WN_TyAbs :
+      forall t, weak_normal (TyAbs t).
+
+Hint Constructors weak_normal.
+
+Inductive well_formed : env -> term -> Prop :=
+  | Wf_NConst :
+      forall G n, 
+        well_formed G (NConst n)
+  | Wf_Add :
+      forall G t1 t2,
+        well_formed G t1 -> well_formed G t2 -> well_formed G (Add t1 t2)
+  | Wf_Var :
+      forall G x T,
+        get G x = Some (term,T) -> well_formed G (Var x)
+  | Wf_Abs :
+      forall G ty t T,
+        well_formed ((term,T) :: G) t -> well_formed G (Abs ty t)
+  | Wf_App :
+      forall G t1 t2,
+        well_formed G t1 -> well_formed G t2 -> well_formed G (App t1 t2) 
+  | Wf_TyAbs :
+      forall G t X,
+        well_formed ((typ,TVar X) :: G) t -> well_formed G (TyAbs t)
+  | Wf_TyApp :
+      forall G X t ty,
+        get G X = Some (typ,TVar X) ->
+        well_formed G t -> well_formed G (TyApp t ty).
+
+Hint Constructors well_formed.
+
+Definition closed (t:term) : Prop := well_formed nil t.
+Definition value (t:term)  : Prop := weak_normal t /\ closed t.
+
+Hint Unfold closed.
+Hint Unfold value.
+
+Reserved Notation "t1 '==>' t2" (at level 40).
+
+Inductive step : term -> term -> Prop :=
+  | EAdd1 :
+      forall t1 t2 t1', 
+        t1 ==> t1' -> 
+        Add t1 t2 ==> Add t1' t2
+  | EAdd2 :
+      forall n t2 t2', 
+        t2 ==> t2' -> 
+        Add (NConst n) t2 ==> Add (NConst n) t2'
+  | EAddPlus :
+      forall n1 n2,
+        Add (NConst n1) (NConst n2) ==> NConst (n1+n2)
+  | EApp1 :
+      forall t1 t2 t1',
+        t1 ==> t1' ->
+        App t1 t2 ==> App t1' t2
+  | EApp2 :
+      forall ty11 t11 t2 t2',
+        t2 ==> t2' ->
+        App (Abs ty11 t11) t2 ==> App (Abs ty11 t11) t2'
+  | EAppAbs :
+      forall ty11 t11 v2,
+        value v2 ->
+        App (Abs ty11 t11) v2 ==> [0 ~> v2] t11
+  | ETyApp :
+      forall t t' ty,
+        t ==> t' ->
+        TyApp t ty ==> TyApp t' ty
+  | ETyAppAbs :
+      forall t11 ty,
+        TyApp (TyAbs t11) ty ==> [0 ~~> ty] t11 
+
+where "t1 '==>' t2" := (step t1 t2).
+
+Hint Constructors step.
+
+(* Next we define a multi step reduction *)
+Reserved Notation "t1 '==>*' t2" (at level 40).
+
+Inductive multi : term -> term -> Prop :=
+  | MRefl : 
+      forall t, 
+        t ==>* t
+  | MStep :
+      forall t1 t2 t3,
+        t1 ==> t2 ->
+        t2 ==>* t3 ->
+        t1 ==>* t3
+
+where "t1 '==>*' t2" := (multi t1 t2).
+
+Hint Constructors multi.
+
+
+Theorem step_deterministic : 
+  forall t1 t2 t3, t1 ==> t2 -> t1 ==> t3 -> t2 = t3.
+Proof.
+  Admitted. (*p
+
+  introh Hs1; generalize dependent t3; induction Hs1; introh Hs2;
+  inverts Hs2; clean 2;
+  try match goal with
+    | [H : forall t', ?T1 ==> _ -> _, H1 : ?T1 ==> _ |- _ ] 
+      => extend (H _ H1); subst; simpl
+  end; 
+  eauto.
+Qed.*)
+
+(* On to typing *)
+
+Reserved Notation "G '||-' t '\:' T" (at level 40).
+
+Inductive type_rel : env -> term -> typ -> Prop :=
+  | TR_NConst :
+      forall G n,
+        G ||- (NConst n) \: TNat
+  | TR_Add :
+      forall G t1 t2,
+        G ||- t1 \: TNat ->
+        G ||- t2 \: TNat ->
+        G ||- (Add t1 t2) \: TNat
+  | TR_Var :
+      forall G x T,
+        get G x = Some (term,T) ->
+        G ||- (Var x) \: T 
+  | TR_Abs :
+      forall G t T1 T2,
+        ((term,T1) :: G) ||- t \: T2 ->
+        G ||- Abs T1 t \: TArrow T1 T2
+  | TR_App :
+      forall G t1 t2 T1 T2,
+        G ||- t1 \: TArrow T1 T2 ->
+        G ||- t2 \: T1 ->
+        G ||- App t1 t2 \: T2
+  | TR_TyAbs :
+      forall G t T,
+        ((typ,0) :: G) ||- t \: T ->
+        G ||- (TyAbs t) \: TAll T
+  | TR_TyApp :
+      forall G t T ty, 
+        G ||- t \: TAll T ->
+        G ||- (TyApp t ty) \: [0 ^> ty] T
+
+where "G '||-' t '\:' T" := (type_rel G t T).
+
+Hint Constructors type_rel.
+
+(* Some type testing *)
+
+Example tc_z  
+  :   nil 
+  ||- TyAbs (Abs (TArrow (TVar 0) (TVar 0)) (Abs (TVar 0) (Var 0))) 
+  \:  TAll (TArrow 
+                 (TArrow (TVar 0) (TVar 0)) 
+                 (TArrow (TVar 0) (TVar 0)))
+  .
+  repeat econstructor; eauto.
+Qed.
+
+Example tc_s  
+  :   nil 
+  ||- TyAbs (Abs (TArrow (TVar 0) (TVar 0)) (Abs (TVar 0) (App (Var 1) (Var 0)))) 
+  \:  TAll (TArrow 
+                 (TArrow (TVar 0) (TVar 0)) 
+                 (TArrow (TVar 0) (TVar 0)))
+  .
+  repeat econstructor; eauto.
+Qed.
+
+Ltac inverts_type :=
+  repeat
+    (match goal with
+       | [ H: _ ||- (NConst _)   \: _ |- _ ] => inverts H
+       | [ H: _ ||- (Add _ _)    \: _ |- _ ] => inverts H
+       | [ H: _ ||- (Var _)      \: _ |- _ ] => inverts H
+       | [ H: _ ||- (Abs _ _)    \: _ |- _ ] => inverts H
+       | [ H: _ ||- (App _ _)    \: _ |- _ ] => inverts H
+       | [ H: _ ||- (TyAbs _)    \: _ |- _ ] => inverts H
+       | [ H: _ ||- (TyApp _ _)  \: _ |- _ ] => inverts H
+     end).
+
+Tactic Notation "induction_type" ident(t) :=
+  induction t; rip; simpl; inverts_type; tburn.
+
+Lemma env_weakening
+  :  forall (G:env)(t:term)(T:typ)(x:var)
+  ,  delete G x ||- t \: T
+  -> G ||- tm_lift x t \: T.
+Proof.
+  rip; gen G T x; induction_type t;
+  match goal with
+    | [ |- context[le_gt_dec ?X ?Y] ] 
+      => break (le_gt_dec X Y); tburn;
+         constructor; rewrite get_delete_above_idx in *; tburn
+  end.
+Qed.
+Hint Resolve env_weakening.
+
+Lemma tm_substition_preserves_typing' 
+  :  forall (G:env)(x:var)(s t:term)(U T:typ)
+  ,  get G x = Some (term,U) 
+  -> delete G x ||- s \: U 
+  -> G ||- t \: T 
+  -> delete G x ||- [x ~> s] t \: T.
+Proof.
+  rip; gen G x s U T; induction_type t;
+  match goal with
+    (* TVar *)
+    | [ |- context [ nat_compare _ _ ] ] 
+      => break_nat_compare; tburn; constructor; tburn
+    (* TAbs *)                                              
+    | [ |- context [ Abs _ ]           ]
+      => econstructor; rewrite delete_rewind; tburn
+  end.
+Qed.
+
+Lemma tm_substition_preserves_typing 
+  :  forall (G:env)(s t:term)(U T:typ)
+  ,  delete ((term,U) :: G) 0 ||- s \: U 
+  -> ((term,U) :: G) ||- t \: T 
+  -> delete ((term,U) :: G) 0 ||- [0 ~> s] t \: T.
+Proof.
+  rip; eapply tm_substition_preserves_typing'; tburn. 
+Qed.
+
+Lemma ty_substition_preserves_typing' 
+  :  forall (G G1 G2:env)(Y X:var)(t:term)(T U:typ)
+  ,  get_split G Y = Some ((typ,TVar X),G1,G2)
+  -> (G1 ++ ((typ,TVar X) :: G2)) ||- t \: T 
+  -> (G1 ++ (delete ((typ,TVar X) :: ([X ^^> U] G2)) 0)) ||- [X ~~> U] t \: [X ^> U] T.
+Proof.
+  rip; gen G X t U T; induction t.
+  Focus 3.
+  
+  
+
+
+
+
+
+
+
+  
+  
+
+Qed.
+
+
+Theorem type_preservation 
+  : forall (t t':term)(T:typ)
+  ,  nil ||- t \: T
+  -> t ==> t'
+  -> nil ||- t' \: T.     
+Proof.
+  rip. gen T t'; induction t; introh Htyp Heval;
+  inverts Htyp; inverts Heval;
+  match goal with
+    | [ |- context[tm_substitute _ _ _] ] 
+      => inverts H2;
+         extend (substition_preserves_typing nil t2 t11 T1 T);
+         simpl in Hextend;
+         apply Hextend; burn
+    | _ => tburn
+  end.
+Qed.
+Hint Resolve type_preservation.
+
+Theorem multi_type_preservation
+  : forall (t t':term)(T:typ)
+  ,  nil ||- t \: T
+  -> t ==>* t'
+  -> nil ||- t' \: T.     
+Proof.
+  introh Htyp Hmult; induction Hmult; burn.
+Qed.
+
+Lemma canonical_forms
+  :  forall (G:env)(t:term)
+  ,  value t
+  (* NConst*)
+  -> (G ||- t \: TNat -> exists n, t = NConst n)
+  (* Abs *)
+  \/ (forall T1 T2
+     ,  G ||- t \: TArrow T1 T2 
+     -> exists t', (T1 :: G) ||- t' \: T2 /\ t = Abs t').
+Proof.
+  rip. unfold value in H. 
+  inversion H. unfold closed in H1.
+  inverts H0.
+
+  burn.
+  inverts H1; burn.
+  inverts H1.
+  right~.
+
+  rip. unfold closed in H2. inverts H0. exists t0. burn.
+Qed.
+
+Lemma nat_canonical_form
+  :  forall (G:env)(t:term)
+  ,  value t 
+  -> G ||- t \: TNat 
+  -> exists n, t = NConst n.
+Proof.
+  rip. unfold value in H. inversion H. unfold closed in H2.
+  inverts H1.
+  burn. clean 2. clean 2.
+Qed.    
+ 
+Lemma abs_canonical_form
+  :  forall (G:env)(t:term)
+  ,  value t
+  -> (forall T1 T2
+     ,  G ||- t \: TArrow T1 T2 
+     -> exists t', (T1 :: G) ||- t' \: T2 /\ t = Abs t').
+Proof.
+  rip. unfold value in H. inverts H. unfold closed in H2.
+  inverts H0. clean 2. inverts H2. burn. clean 2.
+Qed.
+
+Lemma well_typed_imp_well_formed
+  :  forall (G:env)(t:term)(T:typ)
+  ,  G ||- t \: T
+  -> well_formed G t.
+Proof.
+  rip; gen G T; induction_type t.
+Qed.
+
+Theorem type_progress
+  :  forall (t:term)(T:typ)
+  ,  nil ||- t \: T
+  -> value t
+  \/ exists t', t ==> t'.
+Proof.
+  induction_type t.
+  specialize (IHt1 TNat H3). specialize (IHt2 TNat H5).
+  inverts IHt1; inverts IHt2; tburn.
+
+  extend (nat_canonical_form nil t1 H H3). inverts Hextend.
+  extend (nat_canonical_form nil t2 H0 H5). inverts Hextend.
+  burn.
+  extend (nat_canonical_form nil t1 H H3). inverts Hextend.
+  burn.
+
+  left~. unfold value. split~; tburn. unfold closed.
+  econstructor. 
+
+  eapply well_typed_imp_well_formed. eassumption.
+
+  specialize (IHt1 _ H3). specialize (IHt2 _ H5).
+
+  inverts IHt1; inverts IHt2; tburn.
+  extend (abs_canonical_form nil t1 H T1 T H3).
+  inverts Hextend. inverts H1. burn.
+  extend (abs_canonical_form nil t1 H T1 T H3). 
+  inverts Hextend. inverts H1. burn.
+Qed.
+Hint Resolve type_progress.
+
+Theorem type_soundness
+  :  forall (t:term)(T:typ)
+  ,  nil ||- t \: T
+  -> value t 
+  \/ exists t', t ==> t' /\ nil ||- t' \: T.
+Proof.
+  introh Htyp; extend (type_progress t T Htyp); burn.
+Qed.
+
+Theorem multi_type_soundness
+  :  forall (t:term)(T:typ)
+  ,  nil ||- t \: T
+  -> exists t', t ==>* t' /\ value t' /\ nil ||- t' \: T.
+Proof.
+  rip.
+
+
+  
+  
+
+
+
+
+
+
+
+
+
+
+  
+  
+
+                                              
+                                            
