src/Repr/SystemFOp/Term.v
@@ -1,0 +1,246 @@
+Require Import List.
+
+Require Import Repr.Lists.
+
+Require Import Repr.Tactics.All.
+Require Import Repr.Tactics.Rewrite.
+Require Import Repr.Tactics.Burn.
+Require Import Repr.Tactics.Norm.
+Require Import Repr.Tactics.LibTactics.
+
+Require Import Coq.Arith.Peano_dec.
+Require Import Coq.Arith.Compare_dec.
+Require Import Coq.Arith.Lt.
+
+Require Import Repr.SystemFOp.Kind.
+Require Import Repr.SystemFOp.Type.
+
+(* Using var for a de bruijn index states our intent better than nat does *)
+Definition var := nat.
+
+Inductive term : Set :=
+  | NConst : nat -> term
+  | Add    : term -> term -> term
+  | Var    : var -> term
+  | Abs    : typ -> term -> term 
+  | App    : term -> term -> term 
+  | TyAbs  : term -> term
+  | TyApp  : term -> typ -> term .
+Hint Constructors term.
+
+(* Standard de bruijn lifting and substitution operations over terms *)
+Fixpoint term_lift (dp:nat)(t:term) : term :=
+  match t with
+    | NConst n =>
+       NConst n
+    | Add t1 t2 =>
+       Add (term_lift dp t1) (term_lift dp t2)
+    | Var x =>
+       if (le_gt_dec dp x) then Var (S x) else Var x
+    | Abs ty t =>
+       Abs ty (term_lift (S dp) t)
+    | App t1 t2 =>
+       App (term_lift dp t1) (term_lift dp t2) 
+    | TyAbs t =>
+       TyAbs (term_lift dp t)
+    | TyApp t ty =>
+       TyApp (term_lift dp t) ty
+   end.
+
+Fixpoint term_substitute (x:var)(s t:term) : term :=
+  match t with
+    | NConst n => 
+       NConst n
+    | Add t1 t2 => 
+       Add (term_substitute x s t1) (term_substitute x s t2)
+    | Var y => 
+       match nat_compare y x with
+         | Eq => s
+         | Gt => Var (y-1)
+         | Lt => Var y
+       end
+    | Abs ty t' =>
+       Abs ty (term_substitute (S x) (term_lift 0 s) t')
+    | App t1 t2 =>
+       App (term_substitute x s t1) (term_substitute x s t2)
+    | TyAbs t' =>
+       TyAbs (term_substitute x s t')
+    | TyApp t' ty =>
+       TyApp (term_substitute x s t') ty
+  end.
+
+(* Some notation to make our lives easier. *)
+Notation "'[' x '~>' s ']' t" := (term_substitute x s t) (at level 30).
+
+(* We define a weak normal form for terms. *)
+Inductive weak_normal : term -> Prop :=
+  | WN_NConst : 
+      forall n, weak_normal (NConst n)
+  | WN_Var :
+      forall x, weak_normal (Var x)
+  | WN_Abs :
+      forall t ty, weak_normal (Abs ty t) 
+  | WN_TyAbs :
+      forall t, weak_normal (TyAbs t).
+Hint Constructors weak_normal.
+
+(* Terms are well formed with respect to a kind environment and type environment. 
+ * Note that the tricky part is lifting the type environment when a new kind is
+ * pushed onto the kind environment in the TyAbs case. *)
+Inductive well_formed_term : kenv -> tenv -> term -> Prop :=
+  | WF_NConst :
+      forall D G n, 
+        well_formed_term D G (NConst n)
+  | WF_Add :
+      forall D G t1 t2,
+        well_formed_term D G t1 -> 
+        well_formed_term D G t2 -> 
+        well_formed_term D G (Add t1 t2)
+  | WF_Var :
+      forall D G x T,
+        get G x = Some T -> 
+        well_formed_term D G (Var x)
+  | WF_Abs :
+      forall D G ty t T,
+        well_formed_typ D ty ->
+        well_formed_term D (T :: G) t -> 
+        well_formed_term D G (Abs ty t)
+  | WF_App :
+      forall D G t1 t2,
+        well_formed_term D G t1 -> 
+        well_formed_term D G t2 ->
+        well_formed_term D G (App t1 t2) 
+  | WF_TyAbs :
+      forall D G t,
+        well_formed_term (KStar :: D) (tenv_lift 0 G) t ->
+        well_formed_term D G (TyAbs t)
+  | WF_TyApp :
+      forall D G t ty,
+        well_formed_typ D ty ->
+        well_formed_term D G t ->
+        well_formed_term D G (TyApp t ty) .
+Hint Constructors well_formed_term.
+
+(* A term is closed if it is well-formed in the empty kind and type environments. *)
+Definition closed (t:term) : Prop := well_formed_term nil nil t.
+Hint Unfold closed.
+
+(* A closed term is a value if it is in weak normal form. *)
+Definition value (t:term)  : Prop := weak_normal t /\ closed t.
+Hint Unfold value.
+
+(********************************************************************)
+(* We define operational semantics for terms here, and leave the typing
+ * relation to TypeRel.v *)
+
+
+(* Unfortunately, formalizing System F in Coq means we cannot simply overload 
+ * lifting and substition for types over terms. This gets ugly and tedious. *)
+Fixpoint typ_term_lift (dp:nat)(t:term) : term :=
+  match t with
+    | NConst n =>
+       NConst n
+    | Add t1 t2 =>
+       Add (typ_term_lift dp t1) (typ_term_lift dp t2)
+    | Var x =>
+       Var x
+    | Abs ty t =>
+       Abs (typ_lift dp ty) ((typ_term_lift dp) t)
+    | App t1 t2 =>
+       App (typ_term_lift dp t1) (typ_term_lift dp t2) 
+    | TyAbs t =>
+       TyAbs (typ_term_lift (S dp) t)
+    | TyApp t ty =>
+       TyApp (typ_term_lift dp t) (typ_lift dp ty)
+   end.
+
+Fixpoint typ_term_substitute (X:tvar)(U:typ)(t:term) : term :=
+  match t with
+    | NConst n => 
+       NConst n
+    | Add t1 t2 => 
+       Add (typ_term_substitute X U t1) (typ_term_substitute X U t2)
+    | Var x => 
+       Var x
+    | Abs ty t' =>
+       Abs (typ_substitute X U ty) (typ_term_substitute X U t')
+    | App t1 t2 =>
+       App (typ_term_substitute X U t1) (typ_term_substitute X U t2)
+    | TyAbs t' =>
+       TyAbs (typ_term_substitute X U t')
+    | TyApp t' ty =>
+       TyApp (typ_term_substitute X U t') (typ_substitute X U ty)
+  end.
+
+(* Some notation to make our lives easier. *)
+Notation "'[' X '~~>' U ']' t" := (typ_term_substitute X U t) (at level 30).
+
+(* We define a small-step semantics for System F. I prefer a notational definition
+ * when it is obviously what we mean; hence, the '==>'. *)
+Reserved Notation "t1 '==>' t2" (at level 40).
+
+Inductive step : term -> term -> Prop :=
+  | E_Add1 :
+      forall t1 t2 t1', 
+        t1 ==> t1' -> 
+        Add t1 t2 ==> Add t1' t2
+  | E_Add2 :
+      forall n t2 t2', 
+        t2 ==> t2' -> 
+        Add (NConst n) t2 ==> Add (NConst n) t2'
+  | E_AddPlus :
+      forall n1 n2,
+        Add (NConst n1) (NConst n2) ==> NConst (n1+n2)
+  | E_App1 :
+      forall t1 t2 t1',
+        t1 ==> t1' ->
+        App t1 t2 ==> App t1' t2
+  | E_App2 :
+      forall ty11 t11 t2 t2',
+        t2 ==> t2' ->
+        App (Abs ty11 t11) t2 ==> App (Abs ty11 t11) t2'
+  | E_AppAbs :
+      forall ty11 t11 v2,
+        value v2 ->
+        App (Abs ty11 t11) v2 ==> [0 ~> v2] t11
+  | E_TyApp :
+      forall t t' ty,
+        t ==> t' ->
+        TyApp t ty ==> TyApp t' ty
+  | E_TyAppAbs :
+      forall t11 ty,
+        TyApp (TyAbs t11) ty ==> [0 ~~> ty] t11 
+
+where "t1 '==>' t2" := (step t1 t2).
+
+Hint Constructors step.
+
+(* We define a multi step relation mostly for playing around with examples. *)
+Reserved Notation "t1 '==>*' t2" (at level 40).
+
+Inductive multi : term -> term -> Prop :=
+  | MRefl : 
+      forall t, 
+        t ==>* t
+  | MStep :
+      forall t1 t2 t3,
+        t1 ==> t2 ->
+        t2 ==>* t3 ->
+        t1 ==>* t3
+
+where "t1 '==>*' t2" := (multi t1 t2).
+
+Hint Constructors multi.
+
+(********************************************************************)
+
+(* Theorem : Small-step semantics is deterministic. *)
+Theorem step_deterministic 
+  :  forall t1 t2 t3
+  ,  t1 ==> t2 
+  -> t1 ==> t3 
+  -> t2 = t3.
+Proof.
+  introh Hs1; gen t3; induction Hs1; introh Hs2;
+  inverts Hs2; clean 3; tburn.
+Qed.
