src/Repr/SystemFOp/Type.v
@@ -1,0 +1,100 @@
+Require Import List.
+
+Require Import Repr.Lists.
+
+Require Import Repr.Tactics.All.
+Require Import Repr.Tactics.Rewrite.
+Require Import Repr.Tactics.Burn.
+Require Import Repr.Tactics.Norm.
+Require Import Repr.Tactics.LibTactics.
+
+Require Import Coq.Arith.Peano_dec.
+Require Import Coq.Arith.Compare_dec.
+Require Import Coq.Arith.Lt.
+
+Require Import Repr.SystemFOp.Kind.
+
+(* Looks better to use a 'tvar' over a nat for a de bruijn index *)
+Definition tvar := nat.
+
+(* TVars are indexes into a kind environment. We use TNat as our base type. *)
+Inductive typ : Set :=
+  | TVar   : tvar -> typ
+  | TNat   : typ
+  | TArrow : typ -> typ -> typ 
+  | TAll   : typ -> typ .
+
+Hint Constructors typ.
+
+(* Types are well-formed with respect to a kind environment. *)
+Inductive well_formed_typ : kenv -> typ -> Prop :=
+  | WFT_TVar : 
+      forall D X, 
+        (exists K, get D X = Some K) -> 
+        well_formed_typ D (TVar X)
+  | WFT_TNat :
+      forall D, 
+        well_formed_typ D TNat
+  | WFT_TArrow :
+      forall D T1 T2, 
+        well_formed_typ D T1 ->
+        well_formed_typ D T2 ->
+        well_formed_typ D (TArrow T1 T2)
+  | WFT_TAll :
+      forall D K T,
+        well_formed_typ (K :: D) T ->
+        well_formed_typ D (TAll T) .
+
+Hint Constructors well_formed_typ.
+
+(* A type is closed if it is well-formed in the empty kind environment *)
+Definition closed_typ (T:typ) : Prop := well_formed_typ nil T.
+
+(* Standard de bruijn lifting and substituion functions operating at the type level *)
+Fixpoint typ_lift (dp:nat)(T:typ) : typ :=
+  match T with
+    | TVar X =>
+       if (le_gt_dec dp X) then TVar (S X) else TVar X
+    | TNat => 
+       TNat
+    | TArrow T1 T2 =>
+       TArrow (typ_lift dp T1) (typ_lift dp T2)
+    | TAll T' =>
+       TAll (typ_lift (S dp) T')
+  end.
+
+Fixpoint typ_substitute (X:tvar)(U T:typ) : typ :=
+  match T with
+    | TVar Y =>
+       match nat_compare Y X with
+         | Eq => U
+         | Gt => TVar (Y-1)
+         | Lt => TVar Y
+       end
+    | TNat =>
+       TNat
+    | TArrow T1 T2 =>
+       TArrow (typ_substitute X U T1) (typ_substitute X U T2)
+    | TAll T' =>
+       TAll (typ_substitute (S X) (typ_lift 0 U) T')
+  end.
+
+(********************************************************************)
+
+(* We define type environments and some operations over them here. *)
+Definition tenv := list typ.
+Hint Unfold tenv.
+
+(* We will need to lift and substitute over type environments when
+ * new type variables are 'pushed' *)
+Definition tenv_lift (dp:nat)(G:tenv) : tenv := 
+  map (typ_lift dp) G.
+Hint Unfold tenv_lift.
+
+Definition tenv_substitute (X:tvar)(U:typ)(G:tenv) : tenv := 
+  map (typ_substitute X U) G.
+Hint Unfold tenv_substitute.
+
+
+
+
